Use general construction for free state

dm4good/StateFree.v
@@ -1,7 +1,11 @@
 (* Define a partial Dijkstra monad from a free monad for state *)
 
 From Coq Require Import Utf8 RelationClasses.
-From PDM Require Import util PURE.
+From PDM Require Import util guarded PURE PDM StateSpec.
+
+Set Default Goal Selector "!".
+Set Printing Projections.
+Set Universe Polymorphism.
 
 Section State.
 
@@ -37,103 +41,16 @@ Section State.
   Definition reqᴹ (p : Prop) : M p :=
     act_reqᴹ p (λ h, retᴹ h).
 
-  (* Specification monad *)
+  Definition MSt : ReqMonad := {|
+    PDM.M := M ;
+    ret := retᴹ ;
+    bind := bindᴹ ;
+    req := reqᴹ
+  |}.
 
-  Definition preᵂ := state → Prop.
-  Definition postᵂ A := state → A → Prop.
+  (* Effect observation *)
 
-  Definition W A := postᵂ A → preᵂ.
-
-  Definition wle [A] (w₀ w₁ : W A) : Prop :=
-    ∀ P s, w₁ P s → w₀ P s.
-
-  Notation "x ≤ᵂ y" := (wle x y) (at level 80).
-
-  Definition retᵂ [A] (x : A) : W A :=
-    λ P s₀, P s₀ x.
-
-  Definition bindᵂ [A B] (w : W A) (wf : A → W B) : W B :=
-    λ P, w (λ s₁ x, wf x P s₁).
-
-  Definition getᵂ : W state :=
-    λ P s, P s s.
-
-  Definition putᵂ (s : state) : W unit :=
-    λ P s₀, P s tt.
-
-  Definition reqᵂ (p : Prop) : W p :=
-    λ P s₀, ∃ (h : p), P s₀ h.
-
-  Instance trans [A] : Transitive (@wle A).
-  Proof.
-    intros x y z h₁ h₂. intros P s₀ h.
-    apply h₁. apply h₂.
-    assumption.
-  Qed.
-
-  (* Monotonicity *)
-
-  Class Monotonous [A] (w : W A) :=
-    ismono : ∀ (P Q : postᵂ A) s₀, (∀ s₁ x, P s₁ x → Q s₁ x) → w P s₀ → w Q s₀.
-
-  Instance retᵂ_ismono [A] (x : A) : Monotonous (retᵂ x).
-  Proof.
-    intros P Q s₀ hPQ h.
-    apply hPQ. apply h.
-  Qed.
-
-  Instance bindᵂ_ismono [A B] (w : W A) (wf : A → W B) :
-    Monotonous w →
-    (∀ x, Monotonous (wf x)) →
-    Monotonous (bindᵂ w wf).
-  Proof.
-    intros mw mwf.
-    intros P Q s₀ hPQ h.
-    eapply mw. 2: exact h.
-    simpl. intros s₁ x hf.
-    eapply mwf. 2: exact hf.
-    assumption.
-  Qed.
-
-  Instance getᵂ_ismono : Monotonous (getᵂ).
-  Proof.
-    intros P Q s₀ hPQ h.
-    red. red in h.
-    apply hPQ. assumption.
-  Qed.
-
-  Instance putᵂ_ismono : ∀ s, Monotonous (putᵂ s).
-  Proof.
-    intros s. intros P Q s₀ hPQ h.
-    apply hPQ. assumption.
-  Qed.
-
-  Instance reqᵂ_ismono : ∀ p, Monotonous (reqᵂ p).
-  Proof.
-    intros p. intros P Q s₀ hPQ h.
-    destruct h as [hp h].
-    exists hp. apply hPQ. assumption.
-  Qed.
-
-  Lemma bindᵂ_mono :
-    ∀ [A B] (w w' : W A) (wf wf' : A → W B),
-      Monotonous w' →
-      w ≤ᵂ w' →
-      (∀ x, wf x ≤ᵂ wf' x) →
-      bindᵂ w wf ≤ᵂ bindᵂ w' wf'.
-  Proof.
-    intros A B w w' wf wf' mw' hw hwf.
-    intros P s₀ h.
-    red. red in h.
-    apply hw. eapply mw'. 2: exact h.
-    simpl. intros s₁ x hf. apply hwf. assumption.
-  Qed.
-
-  (* Effect observation
-    Here I don't do it in two passes because of the req.
-  *)
-
-  Fixpoint θ [A] (c : M A) : W A :=
+  Fixpoint θ [A] (c : MSt A) : WSt A :=
     match c with
     | retᴹ x => retᵂ x
     | act_getᴹ k => bindᵂ getᵂ (λ x, θ (k x))
@@ -141,66 +58,36 @@ Section State.
     | act_reqᴹ p k => bindᵂ (reqᵂ p) (λ x, θ (k x))
     end.
 
-  Lemma θ_ret :
-    ∀ A (x : A),
-      θ (retᴹ x) ≤ᵂ retᵂ x.
+  Instance θ_morph : LaxMorphism WStOrder θ.
   Proof.
-    intros A x. intros P s₀ h.
-    cbn. red in h. assumption.
-  Qed.
-
-  Lemma θ_bind :
-    ∀ A B c f,
-      θ (@bindᴹ A B c f) ≤ᵂ bindᵂ (θ c) (λ x, θ (f x)).
-  Proof.
-    intros A B c f.
-    induction c as [| ? ih | ?? ih | ?? ih] in B, f |- *.
-    - cbn. intros P s₀ h.
+    constructor.
+    - intros A x. intros P s₀ h.
+      cbn. red in h. assumption.
+    - intros A B c f.
+      induction c as [| ? ih | ?? ih | ?? ih] in B, f |- *.
+      + cbn. intros P s₀ h.
+        assumption.
+      + cbn. intros P s₀ h.
+        apply ih. assumption.
+      + cbn. intros P s₀ h.
+        apply ih. assumption.
+      + cbn. intros P s₀ h.
+        red. red. destruct h as [hp h].
+        exists hp. apply ih. assumption.
+    - intros p. intros post s₀ h.
       assumption.
-    - cbn. intros P s₀ h.
-      apply ih. assumption.
-    - cbn. intros P s₀ h.
-      apply ih. assumption.
-    - cbn. intros P s₀ h.
-      red. red. destruct h as [hp h].
-      exists hp. apply ih. assumption.
   Qed.
 
   (* Partial Dijkstra monad *)
 
-  Definition D A w :=
-    { c : M A | θ c ≤ᵂ w }.
+  Definition D : DijkstraMonad WStOrder :=
+    PDM.D MSt WSt _ WStMono θ θ_morph.
 
-  Definition retᴰ [A] (x : A) : D A (retᵂ x).
-  Proof.
-    exists (retᴹ x).
-    apply θ_ret.
-  Defined.
-
-  Definition bindᴰ [A B w wf] (c : D A w) (f : ∀ x, D B (wf x))
-    `{Monotonous _ w} :
-    D B (bindᵂ w wf).
-  Proof.
-    exists (bindᴹ (val c) (λ x, val (f x))).
-    etransitivity. 1: apply θ_bind.
-    apply bindᵂ_mono.
-    - assumption.
-    - destruct c. assumption.
-    - intro x. destruct (f x). assumption.
-  Qed.
-
-  Definition subcompᴰ [A w w'] (c : D A w) {h : w ≤ᵂ w'} : D A w'.
-  Proof.
-    exists (val c).
-    etransitivity. 2: exact h.
-    destruct c. assumption.
-  Defined.
-
-  Definition getᴰ : D state getᵂ.
+  (* Definition getᴰ : D state getᵂ.
   Proof.
     exists getᴹ.
     cbv. auto.
-  Defined.
+  Defined. *)
 
   Definition putᴰ s : D unit (putᵂ s).
   Proof.
@@ -208,15 +95,9 @@ Section State.
     cbv. auto.
   Defined.
 
-  Definition reqᴰ (p : Prop) : D p (reqᵂ p).
-  Proof.
-    exists (reqᴹ p).
-    cbv. auto.
-  Defined.
-
   (* Lift from PURE *)
 
-  Definition liftᵂ [A] (w : pure_wp A) : W A :=
+  (* Definition liftᵂ [A] (w : pure_wp A) : WSt A.
     λ P s₀, val w (λ x, P s₀ x).
 
   Definition liftᴾ [A w] (f : PURE A w) : D A (liftᵂ w).
@@ -232,6 +113,6 @@ Section State.
     cbv. exists hpre.
     pose proof (prf (f hpre)) as hf. simpl in hf.
     apply hf in h. assumption.
-  Defined.
+  Defined. *)
 
 End State.
